Pushed bitfields all through veric and partway through floyd

floyd/fieldlist.v
@@ -5,6 +5,11 @@ Import compcert.lib.Maps.
 Arguments align !n !amount / .
 Arguments Z.max !n !m / .
 
+Definition plain_member (m: member) : Prop :=
+ match m with Member_plain _ _ => True | _ => False end.
+
+Definition plain_members : members->Prop := Forall plain_member.
+
 Definition field_type i m :=
   match Ctypes.field_type i m with
   | Errors.OK t => t
@@ -13,50 +18,85 @@ Definition field_type i m :=
 
 Definition field_offset env i m :=
   match Ctypes.field_offset env i m with
-  | Errors.OK ofs => ofs
+  | Errors.OK (ofs, Full) => ofs
   | _ => 0
   end.
 
 Fixpoint field_offset_next_rec (env:composite_env) i m ofs sz :=
   match m with
   | nil => 0
-  | (i0, t0) :: m0 =>
+  | m1 :: m0 =>
     match m0 with
     | nil => sz
-    | (_, t1) :: _ =>
-      if ident_eq i i0
-      then align (ofs + @Ctypes.sizeof env t0) (@Ctypes.alignof env t1)
-      else field_offset_next_rec env i m0 (align (ofs + @Ctypes.sizeof env t0) (@Ctypes.alignof env t1)) sz
+    | m2 :: _ =>
+      if ident_eq i (name_member m1)
+      then align (ofs + @Ctypes.sizeof env (type_member m1)) (@Ctypes.alignof env (type_member m2))
+      else field_offset_next_rec env i m0 (align (ofs + @Ctypes.sizeof env (type_member m1)) (@Ctypes.alignof env (type_member m2))) sz
     end
   end.
 
 Definition field_offset_next (env:composite_env) i m sz := field_offset_next_rec env i m 0 sz.
 
-Lemma in_members_field_type: forall i m,
-  in_members i m ->
-  In (i, field_type i m) m.
+Definition in_members i (m: members): Prop :=
+  In i (map name_member m).
+
+Definition members_no_replicate (m: members) : bool :=
+  compute_list_norepet (map name_member m).
+
+Definition compute_in_members id (m: members): bool :=
+  id_in_list id (map name_member m).
+
+Lemma compute_in_members_true_iff: forall i m, compute_in_members i m = true <-> in_members i m.
 Proof.
   intros.
-  unfold field_type.
-  induction m as [|[i0 t0] m].
-  + inversion H.
-  + unfold in_members in H; simpl in H.
-    destruct (ident_eq i0 i).
-    - subst.
-      simpl.
-      if_tac; [| congruence].
-      left. auto.
-    - simpl.
-      right.
-      destruct H; [congruence |].
-      specialize (IHm H).
-      if_tac; [congruence |].
-      exact IHm.
+  unfold compute_in_members.
+  destruct (id_in_list i (map name_member m)) eqn:HH;
+  [apply id_in_list_true in HH | apply id_in_list_false in HH].
+  + unfold in_members.
+    tauto.
+  + unfold in_members; split; [congruence | tauto].
+Qed.
+
+Lemma compute_in_members_false_iff: forall i m,
+  compute_in_members i m = false <-> ~ in_members i m.
+Proof.
+  intros.
+  pose proof compute_in_members_true_iff i m.
+  rewrite <- H; clear H.
+  destruct (compute_in_members i m); split; congruence.
+Qed.
+
+Ltac destruct_in_members i m :=
+  let H := fresh "H" in
+  destruct (compute_in_members i m) eqn:H;
+    [apply compute_in_members_true_iff in H |
+     apply compute_in_members_false_iff in H].
+
+Lemma in_members_dec: forall i m, {in_members i m} + {~ in_members i m}.
+Proof.
+  intros.
+  destruct_in_members i m; [left | right]; auto.
+Qed.
+
+Lemma in_members_field_type: forall i m,
+  plain_members m ->
+  in_members i m ->
+  In (Member_plain i (field_type i m)) m.
+Proof.
+  unfold members_no_replicate, field_type.
+  intros.
+  induction m as [| [|]]; [ | inv H; specialize (IHm H4) .. ].
+  - contradiction H0.
+  -  simpl in *. destruct H0.
+     + subst. left. rewrite if_true by auto. auto. 
+     + if_tac. subst; auto. right. apply IHm; auto.
+  - contradiction.
 Qed.
 
 Lemma field_offset_field_type_match: forall cenv i m,
+  plain_members m ->
   match Ctypes.field_offset cenv i m, Ctypes.field_type i m with
-  | Errors.OK _, Errors.OK _ => True
+  | Errors.OK (_, Full), Errors.OK _ => True
   | Errors.Error _, Errors.Error _ => True
   | _, _ => False
   end.
@@ -64,12 +104,14 @@ Proof.
   intros.
   unfold Ctypes.field_offset.
   remember 0 as pos; clear Heqpos.
-  revert pos; induction m as [| [? ?] ?]; intros.
+  revert pos; induction m; intros.
   + simpl. auto.
-  + simpl. destruct (ident_eq i i0) eqn:HH.
-    - auto.
-    - apply IHm.
-Defined.
+  + inv H. specialize (IHm H3).
+      simpl. if_tac. subst i.
+      destruct a; simpl. auto.
+      inv H2.
+      apply IHm.
+Qed.
 
 Lemma field_type_in_members: forall i m,
   match Ctypes.field_type i m with
@@ -79,10 +121,10 @@ Lemma field_type_in_members: forall i m,
 Proof.
   intros.
   unfold in_members.
-  induction m as [| [i0 t0] m].
+  induction m.
   + simpl; tauto.
   + simpl.
-    destruct (ident_eq i i0).
+     if_tac.
     - left; subst; auto.
     - destruct (Ctypes.field_type i m).
       * right; auto.
@@ -92,24 +134,24 @@ Qed.
 Section COMPOSITE_ENV.
 Context {cs: compspecs}.
 
-Ltac solve_field_offset_type i m :=
+Ltac solve_field_offset_type i m PLAIN :=
   let H := fresh "H" in
   let Hty := fresh "H" in
   let Hofs := fresh "H" in
   let t := fresh "t" in
   let ofs := fresh "ofs" in
-  pose proof field_offset_field_type_match cenv_cs i m;
-  destruct (Ctypes.field_offset cenv_cs i m) as [ofs|?] eqn:Hofs, (Ctypes.field_type i m) as [t|?] eqn:Hty;
-    [clear H | inversion H | inversion H | clear H].
+  assert (H := field_offset_field_type_match cenv_cs i m PLAIN);
+  destruct (Ctypes.field_offset cenv_cs i m) as [[ofs [|]]|?] eqn:Hofs, (Ctypes.field_type i m) as [t|?] eqn:Hty;
+   [clear H | inversion H | inversion H | inversion H | inversion H | clear H ].
 
-Lemma complete_legal_cosu_member: forall (cenv : composite_env) (id : ident) (t : type) (m : list (ident * type)),
-  In (id, t) m -> @composite_complete_legal_cosu_type cenv m = true -> @complete_legal_cosu_type cenv t = true.
+Lemma complete_legal_cosu_member: forall (cenv : composite_env) (id : ident) (t : type) (m : members),
+  In (Member_plain id t) m -> @composite_complete_legal_cosu_type cenv m = true -> @complete_legal_cosu_type cenv t = true.
 Proof.
   intros.
-  induction m as [| [i0 t0] ?].
+  induction m.
   + inv H.
-  + destruct H.
-    - inv H.
+  + destruct H. subst.
+    - 
       simpl in H0.
       rewrite andb_true_iff in H0; tauto.
     - apply IHm; auto.
@@ -117,20 +159,23 @@ Proof.
       rewrite andb_true_iff in H0; tauto.
 Qed.         
 
-Lemma complete_legal_cosu_type_field_type: forall id i,
+Lemma complete_legal_cosu_type_field_type: forall id i
+  (PLAIN: plain_members (co_members (get_co id))),
   in_members i (co_members (get_co id)) ->
   complete_legal_cosu_type (field_type i (co_members (get_co id))) = true.
 Proof.
   unfold get_co.
   intros.
   destruct (cenv_cs ! id) as [co |] eqn:CO.
-  + apply in_members_field_type in H.
+  + apply in_members_field_type in H; auto.
     pose proof cenv_legal_su _ _ CO.
     eapply complete_legal_cosu_member; eauto.
   + inversion H.
 Qed.
 
-Lemma align_compatible_rec_Tstruct_inv': forall id a ofs,
+Lemma align_compatible_rec_Tstruct_inv': forall id
+  (PLAIN: plain_members (co_members (get_co id)))
+  a ofs,
   align_compatible_rec cenv_cs (Tstruct id a) ofs ->
   forall i,
   in_members i (co_members (get_co id)) ->
@@ -142,17 +187,19 @@ Proof.
   destruct (cenv_cs ! id) as [co |] eqn:CO.
   + eapply align_compatible_rec_Tstruct_inv with (i0 := i); try eassumption.
     - unfold field_type.
-      induction (co_members co) as [| [i0 t0] ?].
+      induction (co_members co).
       * inv H0.
       * simpl; if_tac; auto.
-        apply IHm.
+        apply IHm. inv PLAIN; auto.
         destruct H0; [simpl in H0; congruence | auto].
     - unfold field_offset, Ctypes.field_offset.
       generalize 0 at 1 2.
-      induction (co_members co) as [| [i0 t0] ?]; intros.
+      induction (co_members co); intros.
       * inv H0.
-      * simpl; if_tac; auto.
-        apply IHm.
+      * unfold field_offset_rec; fold field_offset_rec.
+        inv PLAIN. destruct a0; try contradiction. simpl.
+        if_tac; auto.
+        apply IHm; auto.
         destruct H0; [simpl in H0; congruence | auto].
   + inv H0.
 Qed.
@@ -168,7 +215,7 @@ Proof.
   destruct (cenv_cs ! id) as [co |] eqn:CO.
   + eapply align_compatible_rec_Tunion_inv with (i0 := i); try eassumption.
     unfold field_type.
-    induction (co_members co) as [| [i0 t0] ?].
+    induction (co_members co).
     - inv H0.
     - simpl; if_tac; auto.
       apply IHm.
@@ -180,61 +227,75 @@ Lemma field_offset_aligned: forall i m,
   (alignof (field_type i m) | field_offset cenv_cs i m).
 Proof.
   intros.
-  unfold field_type, field_offset.
-  solve_field_offset_type i m.
-  + eapply field_offset_aligned; eauto.
-  + apply Z.divide_0_r.
+ unfold field_offset. unfold field_type.
+  destruct (Ctypes.field_offset cenv_cs i m) as [[? [|]]|] eqn:?H.
+  destruct (Ctypes.field_type i m) eqn:?H.
+ apply (field_offset_aligned cenv_cs i m _ _ H H0).
+ apply Z.divide_1_l.
+ apply Z.divide_0_r.
+ apply Z.divide_0_r.
 Qed.
 
-Lemma alignof_composite_hd_divide: forall i t m, (alignof t | alignof_composite cenv_cs ((i, t) :: m)).
+Lemma alignof_composite_hd_divide: forall m1 m
+  (PLAIN: plain_members (m1::m)),
+  (alignof (type_member m1) | alignof_composite cenv_cs (m1 :: m)).
 Proof.
   intros.
-  destruct (alignof_two_p t) as [N ?].
-  destruct (alignof_composite_two_p cenv_cs ((i, t) :: m)) as [M ?].
-  assert (alignof t <= alignof_composite cenv_cs ((i,t)::m)) by (apply Z.le_max_l).
+  inv PLAIN.
+  destruct (alignof_composite_two_p cenv_cs (m1 :: m)) as [M H0].
+  destruct m1; inv H1.
+  simpl.
+  destruct (alignof_two_p t) as [N H].
+  assert (alignof t <= alignof_composite cenv_cs (Member_plain id t :: m)) by apply Z.le_max_l.
   fold (alignof t) in H.
   rewrite H in *.
+  simpl in *.
   rewrite H0 in *.
   exact (power_nat_divide N M H1).
 Qed.
 
-Lemma alignof_composite_tl_divide: forall i t m, (alignof_composite cenv_cs m | alignof_composite cenv_cs ((i, t) :: m)).
+Lemma alignof_composite_tl_divide: forall m1 m
+  (PLAIN: plain_members (m1::m)),
+   (alignof_composite cenv_cs m | alignof_composite cenv_cs (m1 :: m)).
 Proof.
   intros.
   destruct (alignof_composite_two_p cenv_cs m) as [N ?].
-  destruct (alignof_composite_two_p cenv_cs ((i, t) :: m)) as [M ?].
-  assert (alignof_composite cenv_cs m <= alignof_composite cenv_cs ((i, t) :: m)) by (apply Z.le_max_r).
+  destruct (alignof_composite_two_p cenv_cs (m1 :: m)) as [M ?].
+  inv PLAIN. destruct m1; inv H3.
+  assert (alignof_composite cenv_cs m <= alignof_composite cenv_cs (Member_plain id t :: m)) by (apply Z.le_max_r).
   rewrite H in *.
   rewrite H0 in *.
   exact (power_nat_divide N M H1).
 Qed.
 
-Lemma alignof_field_type_divide_alignof: forall i m,
+Lemma alignof_field_type_divide_alignof: forall i m
+  (PLAIN: plain_members m),
   in_members i m ->
   (alignof (field_type i m) | alignof_composite cenv_cs m).
 Proof.
   intros.
   unfold field_type.
-  induction m as [| [i0 t0] m].
+  induction m. 
   + inversion H.
   + unfold in_members in H; simpl in H.
     simpl Ctypes.field_type.
     if_tac.
-    - apply alignof_composite_hd_divide.
+    - apply alignof_composite_hd_divide; auto.
     - eapply Z.divide_trans.
-      * apply IHm.
+      * inv PLAIN. apply IHm; auto.
         destruct H; [congruence | auto].
-      * apply alignof_composite_tl_divide.
+      * apply alignof_composite_tl_divide; auto.
 Qed.
 
 (* if sizeof Tvoid = 0, this lemma can be nicer. *)
-Lemma field_offset_in_range: forall i m,
+Lemma field_offset_in_range: forall i m
+  (PLAIN: plain_members m),
   in_members i m ->
-  0 <= field_offset cenv_cs i m /\ field_offset cenv_cs i m + sizeof (field_type i m) <= sizeof_struct cenv_cs 0 m.
+  0 <= field_offset cenv_cs i m /\ field_offset cenv_cs i m + sizeof (field_type i m) <= sizeof_struct cenv_cs m.
 Proof.
   intros.
   unfold field_offset, field_type.
-  solve_field_offset_type i m.
+  solve_field_offset_type i m PLAIN.
   + eapply field_offset_in_range; eauto.
   + pose proof field_type_in_members i m.
     rewrite H1 in H0.
@@ -250,21 +311,22 @@ Proof.
   intros.
   unfold in_members in H.
   unfold field_type.
-  induction m as [|[i0 t0] m].
+  induction m.
   + inversion H.
   + simpl.
-    destruct (ident_eq i i0).
+    destruct (ident_eq i (name_member a)).
     - apply Z.le_max_l.
     - simpl in H; destruct H; [congruence |].
      specialize (IHm H).
-     fold (sizeof t0).
-     pose proof Z.le_max_r (sizeof t0) (sizeof_union cenv_cs m).
+     fold (sizeof (type_member a)).
+     pose proof Z.le_max_r (sizeof (type_member a)) (sizeof_union cenv_cs m).
      lia.
 Qed.
 
 (* if sizeof Tvoid = 0, this lemma can be nicer. *)
 Lemma field_offset_no_overlap:
-  forall i1 i2 m,
+  forall i1 i2 m
+  (PLAIN: plain_members m),
   i1 <> i2 ->
   in_members i1 m ->
   in_members i2 m ->
@@ -275,9 +337,10 @@ Proof.
   unfold field_offset, field_type.
   pose proof field_type_in_members i1 m.
   pose proof field_type_in_members i2 m.
-  solve_field_offset_type i1 m;
-  solve_field_offset_type i2 m; try tauto.
-  eapply field_offset_no_overlap; eauto.
+  solve_field_offset_type i1 m PLAIN;
+  solve_field_offset_type i2 m PLAIN; try tauto.
+ pose proof (field_offset_no_overlap _ _ _ _ _ _ _ _ _ _ H6 H5 H8 H7 H).
+  unfold layout_start, layout_width, bitsizeof in H4. unfold sizeof. lia.
 Qed.
 
 Lemma not_in_members_field_type: forall i m,
@@ -286,11 +349,11 @@ Lemma not_in_members_field_type: forall i m,
 Proof.
   unfold in_members, field_type.
   intros.
-  induction m as [| [i0 t0] m].
+  induction m.
   + reflexivity.
   + simpl in H.
     simpl.
-    destruct (ident_eq i i0) as [HH | HH]; pose proof (@eq_sym ident i i0); tauto.
+    destruct (ident_eq i (name_member a)) as [HH | HH]; pose proof (@eq_sym ident i (name_member a)); tauto.
 Qed.
 
 Lemma not_in_members_field_offset: forall i m,
@@ -300,45 +363,96 @@ Proof.
   unfold in_members, field_offset, Ctypes.field_offset.
   intros.
   generalize 0 at 1.
-  induction m as [| [i0 t0] m]; intros.
+  induction m; intros.
   + reflexivity.
   + simpl in H.
     simpl.
-    destruct (ident_eq i i0) as [HH | HH]; pose proof (@eq_sym ident i i0); [tauto |].
+    destruct (ident_eq i _) as [HH | HH]; pose proof (@eq_sym ident i (name_member a)); [tauto |].
     apply IHm. tauto.
 Qed.
 
-Lemma field_offset_next_in_range: forall i m sz,
+Lemma align_bitalign: (* copied from veric/align_mem.v *)
+  forall z a, a > 0 ->
+    align z a = align (z * 8) (a * 8) / 8.
+Proof.
+clear.
+intros.  unfold align.
+rewrite Z.mul_assoc.
+rewrite Z.div_mul by congruence.
+f_equal.
+transitivity ((z + a - 1)*8 / (a*8)).
+rewrite Z.div_mul_cancel_r by lia; auto.
+rewrite! Z.add_sub_swap.
+rewrite Z.mul_add_distr_r.
+assert (H0: ((z - 1) * 8 + 1*(a * 8)) / (a * 8) = (z * 8 - 1 + 1*(a * 8)) / (a * 8))
+ ; [ | rewrite Z.mul_1_l in H0; auto].
+rewrite !Z.div_add by lia.
+f_equal.
+rewrite Z.mul_sub_distr_r.
+rewrite Z.mul_1_l.
+rewrite (Z.mul_comm a).
+rewrite <- !Zdiv.Zdiv_Zdiv by lia.
+f_equal.
+transitivity (((z-1)*8)/8).
+f_equal; lia.
+rewrite Z.div_mul by lia.
+rewrite <- !(Z.add_opp_r (_ * _)).
+rewrite Z.div_add_l by lia.
+reflexivity.
+Qed.
+
+Lemma field_offset_next_in_range: forall i m sz
+  (PLAIN: plain_members m),
   in_members i m ->
-  sizeof_struct cenv_cs 0 m <= sz ->
+  sizeof_struct cenv_cs m <= sz ->
   field_offset cenv_cs i m + sizeof (field_type i m) <=
   field_offset_next cenv_cs i m sz <= sz.
 Proof.
   intros.
-  destruct m as [| [i0 t0] m]; [inversion H |].
+  destruct m as [| m1 m]; [inversion H |].
+  unfold sizeof_struct in H0.
   unfold field_offset, Ctypes.field_offset, field_offset_next, field_type.
-  pattern 0 at 3 4; replace 0 with (align 0 (alignof t0)) by (apply align_0, alignof_pos).
+  pattern 0 at 4 5; replace 0 with (align (0*8) (alignof (type_member m1))) by (apply align_0, alignof_pos).
   match goal with
   | |- ?A => assert (A /\
-                     match field_offset_rec cenv_cs i ((i0, t0) :: m) 0 with
+                     match field_offset_rec cenv_cs i (m1 :: m) 0 with
                      | Errors.OK _ => True
                      | _ => False
                      end /\
-                     match Ctypes.field_type i ((i0, t0) :: m) with
+                     match Ctypes.field_type i (m1 :: m) with
                      | Errors.OK _ => True
                      | _ => False
                      end); [| tauto]
   end.
-  revert i0 t0 H H0; generalize 0; induction m as [| [i1 t1] m]; intros.
-  + destruct (ident_eq i i0); [| destruct H; simpl in H; try congruence; tauto].
+  inv PLAIN. rename H4 into PLAIN. rename H3 into PLAIN1.
+  rewrite <- (Z.mul_0_l 8) in H0.
+ change (field_offset_rec cenv_cs i (m1::m) 0) with (field_offset_rec cenv_cs i (m1::m) (0*8)).
+  revert m1 PLAIN1 H H0; generalize 0.
+  induction m as [| m0 m]; intros.
+  + destruct (ident_eq i (name_member m1)); [| destruct H; simpl in H; try congruence; tauto].
     subst; simpl.
-    if_tac; [| congruence].
+    rewrite !if_true by auto.
+    destruct m1; inv PLAIN1. simpl in *.
     split; [| split]; auto.
-    simpl in H0.
-   fold (sizeof t0) in *.
-    lia.
-  + remember ((i1, t1) :: m) as m0. simpl in H0 |- *. subst m0.
-    destruct (ident_eq i i0).
+    unfold bitalignof, bitsizeof, bytes_of_bits in *.
+    split; [ | lia].
+    eapply Z.le_trans; try apply H0. clear H0.
+    rewrite <- (Z.div_mul (sizeof t) 8) by computable.
+    pose proof (sizeof_pos t).
+    fold (sizeof t). forget (sizeof t) as s.
+    pose proof (Ctypes.alignof_pos t).
+    forget (Ctypes.alignof t) as a. 
+     unfold align.
+    replace (z*8 + a*8 - 1) with ((z*8-1)+1*(a*8)) by lia.
+    rewrite Z.div_add by lia.
+    replace (((z * 8 - 1) / (a * 8) + 1) * (a * 8)  + s*8 + 7) with (((z * 8 - 1) / (a * 8) + 1) * (a * 8)  + 7 + s*8) by lia.
+    rewrite Z.div_add by lia.
+    rewrite Z.div_mul by lia.
+    apply Zplus_le_compat_r.
+    apply Z.div_le_mono. computable. lia.
+  + remember (m0::m) as m0'.  simpl in H0 |- *. subst m0'.
+     destruct m1; inv PLAIN1. simpl in *.
+     if_tac.
     - split; [| split]; auto.
       split.
       * apply align_le, alignof_pos.
