veric/mpred.v
@@ -228,47 +228,6 @@ Definition int_range (sz: intsize) (sgn: signedness) (i: int) :=
  | IBool, _ => 0 <= Int.unsigned i < 256
  end.
 
-Definition in_members i (m: members): Prop :=
-  In i (map name_member m).
-
-Definition members_no_replicate (m: members) : bool :=
-  compute_list_norepet (map name_member m).
-
-Definition compute_in_members id (m: members): bool :=
-  id_in_list id (map name_member m).
-
-Lemma compute_in_members_true_iff: forall i m, compute_in_members i m = true <-> in_members i m.
-Proof.
-  intros.
-  unfold compute_in_members.
-  destruct (id_in_list i (map name_member m)) eqn:HH;
-  [apply id_in_list_true in HH | apply id_in_list_false in HH].
-  + unfold in_members.
-    tauto.
-  + unfold in_members; split; [congruence | tauto].
-Qed.
-
-Lemma compute_in_members_false_iff: forall i m,
-  compute_in_members i m = false <-> ~ in_members i m.
-Proof.
-  intros.
-  pose proof compute_in_members_true_iff i m.
-  rewrite <- H; clear H.
-  destruct (compute_in_members i m); split; congruence.
-Qed.
-
-Ltac destruct_in_members i m :=
-  let H := fresh "H" in
-  destruct (compute_in_members i m) eqn:H;
-    [apply compute_in_members_true_iff in H |
-     apply compute_in_members_false_iff in H].
-
-Lemma in_members_dec: forall i m, {in_members i m} + {~ in_members i m}.
-Proof.
-  intros.
-  destruct_in_members i m; [left | right]; auto.
-Qed.
-
 Lemma size_chunk_sizeof: forall env t ch, access_mode t = By_value ch -> sizeof env t = Memdata.size_chunk ch.
 Proof.
   intros.
@@ -278,6 +237,9 @@ Proof.
   - destruct f; inversion H1; reflexivity.
   - inversion H1; reflexivity.
 Qed.
+
+Definition members_no_replicate (m: members) : bool :=
+  compute_list_norepet (map name_member m).
 
 Definition composite_legal_fieldlist (co: composite): Prop :=
   members_no_replicate (co_members co) = true.
