progs/objectSelfFancy.v
@@ -1,10 +1,12 @@
 From Coq Require Import String List ZArith.
 From compcert Require Import Coqlib Integers Floats AST Ctypes Cop Clight Clightdefs.
+Import Clightdefs.ClightNotations.
 Local Open Scope Z_scope.
 Local Open Scope string_scope.
+Local Open Scope clight_scope.
 
 Module Info.
-  Definition version := "3.8".
+  Definition version := "3.9".
   Definition build_number := "".
   Definition build_tag := "".
   Definition build_branch := "".
@@ -29,101 +31,103 @@ Definition ___builtin_clzll : ident := 20%positive.
 Definition ___builtin_ctz : ident := 21%positive.
 Definition ___builtin_ctzl : ident := 22%positive.
 Definition ___builtin_ctzll : ident := 23%positive.
-Definition ___builtin_debug : ident := 66%positive.
+Definition ___builtin_debug : ident := 49%positive.
+Definition ___builtin_expect : ident := 38%positive.
 Definition ___builtin_fabs : ident := 24%positive.
 Definition ___builtin_fabsf : ident := 25%positive.
-Definition ___builtin_fmadd : ident := 58%positive.
-Definition ___builtin_fmax : ident := 56%positive.
-Definition ___builtin_fmin : ident := 57%positive.
-Definition ___builtin_fmsub : ident := 59%positive.
-Definition ___builtin_fnmadd : ident := 60%positive.
-Definition ___builtin_fnmsub : ident := 61%positive.
+Definition ___builtin_fmadd : ident := 41%positive.
+Definition ___builtin_fmax : ident := 39%positive.
+Definition ___builtin_fmin : ident := 40%positive.
+Definition ___builtin_fmsub : ident := 42%positive.
+Definition ___builtin_fnmadd : ident := 43%positive.
+Definition ___builtin_fnmsub : ident := 44%positive.
 Definition ___builtin_fsqrt : ident := 26%positive.
 Definition ___builtin_membar : ident := 32%positive.
 Definition ___builtin_memcpy_aligned : ident := 28%positive.
-Definition ___builtin_read16_reversed : ident := 62%positive.
-Definition ___builtin_read32_reversed : ident := 63%positive.
+Definition ___builtin_read16_reversed : ident := 45%positive.
+Definition ___builtin_read32_reversed : ident := 46%positive.
 Definition ___builtin_sel : ident := 29%positive.
 Definition ___builtin_sqrt : ident := 27%positive.
+Definition ___builtin_unreachable : ident := 37%positive.
 Definition ___builtin_va_arg : ident := 34%positive.
 Definition ___builtin_va_copy : ident := 35%positive.
 Definition ___builtin_va_end : ident := 36%positive.
 Definition ___builtin_va_start : ident := 33%positive.
-Definition ___builtin_write16_reversed : ident := 64%positive.
-Definition ___builtin_write32_reversed : ident := 65%positive.
-Definition ___compcert_i64_dtos : ident := 41%positive.
-Definition ___compcert_i64_dtou : ident := 42%positive.
-Definition ___compcert_i64_sar : ident := 53%positive.
-Definition ___compcert_i64_sdiv : ident := 47%positive.
-Definition ___compcert_i64_shl : ident := 51%positive.
-Definition ___compcert_i64_shr : ident := 52%positive.
-Definition ___compcert_i64_smod : ident := 49%positive.
-Definition ___compcert_i64_smulh : ident := 54%positive.
-Definition ___compcert_i64_stod : ident := 43%positive.
-Definition ___compcert_i64_stof : ident := 45%positive.
-Definition ___compcert_i64_udiv : ident := 48%positive.
-Definition ___compcert_i64_umod : ident := 50%positive.
-Definition ___compcert_i64_umulh : ident := 55%positive.
-Definition ___compcert_i64_utod : ident := 44%positive.
-Definition ___compcert_i64_utof : ident := 46%positive.
-Definition ___compcert_va_composite : ident := 40%positive.
-Definition ___compcert_va_float64 : ident := 39%positive.
-Definition ___compcert_va_int32 : ident := 37%positive.
-Definition ___compcert_va_int64 : ident := 38%positive.
-Definition _c : ident := 79%positive.
-Definition _col : ident := 91%positive.
-Definition _colU : ident := 96%positive.
+Definition ___builtin_write16_reversed : ident := 47%positive.
+Definition ___builtin_write32_reversed : ident := 48%positive.
+Definition ___compcert_i64_dtos : ident := 85%positive.
+Definition ___compcert_i64_dtou : ident := 86%positive.
+Definition ___compcert_i64_sar : ident := 97%positive.
+Definition ___compcert_i64_sdiv : ident := 91%positive.
+Definition ___compcert_i64_shl : ident := 95%positive.
+Definition ___compcert_i64_shr : ident := 96%positive.
+Definition ___compcert_i64_smod : ident := 93%positive.
+Definition ___compcert_i64_smulh : ident := 98%positive.
+Definition ___compcert_i64_stod : ident := 87%positive.
+Definition ___compcert_i64_stof : ident := 89%positive.
+Definition ___compcert_i64_udiv : ident := 92%positive.
+Definition ___compcert_i64_umod : ident := 94%positive.
+Definition ___compcert_i64_umulh : ident := 99%positive.
+Definition ___compcert_i64_utod : ident := 88%positive.
+Definition ___compcert_i64_utof : ident := 90%positive.
+Definition ___compcert_va_composite : ident := 84%positive.
+Definition ___compcert_va_float64 : ident := 83%positive.
+Definition ___compcert_va_int32 : ident := 81%positive.
+Definition ___compcert_va_int64 : ident := 82%positive.
+Definition _c : ident := 62%positive.
+Definition _col : ident := 74%positive.
+Definition _colU : ident := 79%positive.
 Definition _color : ident := 12%positive.
-Definition _d : ident := 72%positive.
+Definition _d : ident := 55%positive.
 Definition _data : ident := 7%positive.
-Definition _exit : ident := 68%positive.
-Definition _fancyfoo_methods : ident := 80%positive.
+Definition _exit : ident := 51%positive.
+Definition _fancyfoo_methods : ident := 63%positive.
 Definition _fancyfoo_object : ident := 13%positive.
 Definition _fancymethods : ident := 11%positive.
-Definition _foo_methods : ident := 76%positive.
+Definition _foo_methods : ident := 59%positive.
 Definition _foo_object : ident := 8%positive.
-Definition _foo_reset : ident := 70%positive.
-Definition _foo_twiddle : ident := 73%positive.
-Definition _foo_twiddleR : ident := 75%positive.
+Definition _foo_reset : ident := 53%positive.
+Definition _foo_twiddle : ident := 56%positive.
+Definition _foo_twiddleR : ident := 58%positive.
 Definition _getcolor : ident := 10%positive.
-Definition _i : ident := 71%positive.
-Definition _main : ident := 97%positive.
-Definition _make_fancyfoo : ident := 81%positive.
-Definition _make_fancyfooTyped : ident := 82%positive.
-Definition _make_foo : ident := 78%positive.
-Definition _malloc : ident := 67%positive.
+Definition _i : ident := 54%positive.
+Definition _main : ident := 80%positive.
+Definition _make_fancyfoo : ident := 64%positive.
+Definition _make_fancyfooTyped : ident := 65%positive.
+Definition _make_foo : ident := 61%positive.
+Definition _malloc : ident := 50%positive.
 Definition _methods : ident := 5%positive.
 Definition _mtable : ident := 6%positive.
-Definition _object : ident := 1%positive.
-Definition _p : ident := 77%positive.
-Definition _p_reset : ident := 84%positive.
-Definition _p_twiddle : ident := 85%positive.
-Definition _pmtable : ident := 83%positive.
-Definition _q : ident := 86%positive.
-Definition _q_getcolor : ident := 90%positive.
-Definition _q_reset : ident := 88%positive.
-Definition _q_setcolor : ident := 89%positive.
-Definition _qmtable : ident := 87%positive.
-Definition _reset : ident := 2%positive.
-Definition _s_reset : ident := 74%positive.
-Definition _self : ident := 69%positive.
+Definition _object : ident := 2%positive.
+Definition _p : ident := 60%positive.
+Definition _p_reset : ident := 67%positive.
+Definition _p_twiddle : ident := 68%positive.
+Definition _pmtable : ident := 66%positive.
+Definition _q : ident := 69%positive.
+Definition _q_getcolor : ident := 73%positive.
+Definition _q_reset : ident := 71%positive.
+Definition _q_setcolor : ident := 72%positive.
+Definition _qmtable : ident := 70%positive.
+Definition _reset : ident := 1%positive.
+Definition _s_reset : ident := 57%positive.
+Definition _self : ident := 52%positive.
 Definition _setcolor : ident := 9%positive.
 Definition _twiddle : ident := 3%positive.
 Definition _twiddleR : ident := 4%positive.
-Definition _u : ident := 92%positive.
-Definition _u_getcolor : ident := 95%positive.
-Definition _u_reset : ident := 94%positive.
-Definition _umtable : ident := 93%positive.
-Definition _t'1 : ident := 98%positive.
-Definition _t'10 : ident := 107%positive.
-Definition _t'2 : ident := 99%positive.
-Definition _t'3 : ident := 100%positive.
-Definition _t'4 : ident := 101%positive.
-Definition _t'5 : ident := 102%positive.
-Definition _t'6 : ident := 103%positive.
-Definition _t'7 : ident := 104%positive.
-Definition _t'8 : ident := 105%positive.
-Definition _t'9 : ident := 106%positive.
+Definition _u : ident := 75%positive.
+Definition _u_getcolor : ident := 78%positive.
+Definition _u_reset : ident := 77%positive.
+Definition _umtable : ident := 76%positive.
+Definition _t'1 : ident := 100%positive.
+Definition _t'10 : ident := 109%positive.
+Definition _t'2 : ident := 101%positive.
+Definition _t'3 : ident := 102%positive.
+Definition _t'4 : ident := 103%positive.
+Definition _t'5 : ident := 104%positive.
+Definition _t'6 : ident := 105%positive.
+Definition _t'7 : ident := 106%positive.
+Definition _t'8 : ident := 107%positive.
+Definition _t'9 : ident := 108%positive.
 
 Definition f_foo_reset := {|
   fn_return := tvoid;
@@ -673,51 +677,138 @@ Definition f_main := {|
 
 Definition composites : list composite_definition :=
 (Composite _methods Struct
-   ((_reset,
-     (tptr (Tfunction (Tcons (tptr (Tstruct _object noattr)) Tnil) tvoid
-             cc_default))) ::
-    (_twiddle,
-     (tptr (Tfunction
-             (Tcons (tptr (Tstruct _object noattr)) (Tcons tint Tnil)) tint
-             cc_default))) ::
-    (_twiddleR,
-     (tptr (Tfunction
-             (Tcons (tptr (Tstruct _object noattr)) (Tcons tint Tnil)) tint
-             cc_default))) :: nil)
+   (Member_plain _reset
+      (tptr (Tfunction (Tcons (tptr (Tstruct _object noattr)) Tnil) tvoid
+              cc_default)) ::
+    Member_plain _twiddle
+      (tptr (Tfunction
+              (Tcons (tptr (Tstruct _object noattr)) (Tcons tint Tnil)) tint
+              cc_default)) ::
+    Member_plain _twiddleR
+      (tptr (Tfunction
+              (Tcons (tptr (Tstruct _object noattr)) (Tcons tint Tnil)) tint
+              cc_default)) :: nil)
    noattr ::
  Composite _object Struct
-   ((_mtable, (tptr (Tstruct _methods noattr))) :: nil)
+   (Member_plain _mtable (tptr (Tstruct _methods noattr)) :: nil)
    noattr ::
  Composite _foo_object Struct
-   ((_mtable, (tptr (Tstruct _methods noattr))) :: (_data, tint) :: nil)
+   (Member_plain _mtable (tptr (Tstruct _methods noattr)) ::
+    Member_plain _data tint :: nil)
    noattr ::
  Composite _fancymethods Struct
-   ((_reset,
-     (tptr (Tfunction (Tcons (tptr (Tstruct _object noattr)) Tnil) tvoid
-             cc_default))) ::
-    (_twiddle,
-     (tptr (Tfunction
-             (Tcons (tptr (Tstruct _object noattr)) (Tcons tint Tnil)) tint
-             cc_default))) ::
-    (_twiddleR,
-     (tptr (Tfunction
-             (Tcons (tptr (Tstruct _object noattr)) (Tcons tint Tnil)) tint
-             cc_default))) ::
-    (_setcolor,
-     (tptr (Tfunction
-             (Tcons (tptr (Tstruct _object noattr)) (Tcons tint Tnil)) tvoid
-             cc_default))) ::
-    (_getcolor,
-     (tptr (Tfunction (Tcons (tptr (Tstruct _object noattr)) Tnil) tint
-             cc_default))) :: nil)
+   (Member_plain _reset
+      (tptr (Tfunction (Tcons (tptr (Tstruct _object noattr)) Tnil) tvoid
+              cc_default)) ::
+    Member_plain _twiddle
+      (tptr (Tfunction
+              (Tcons (tptr (Tstruct _object noattr)) (Tcons tint Tnil)) tint
+              cc_default)) ::
+    Member_plain _twiddleR
+      (tptr (Tfunction
+              (Tcons (tptr (Tstruct _object noattr)) (Tcons tint Tnil)) tint
+              cc_default)) ::
+    Member_plain _setcolor
+      (tptr (Tfunction
+              (Tcons (tptr (Tstruct _object noattr)) (Tcons tint Tnil)) tvoid
+              cc_default)) ::
+    Member_plain _getcolor
+      (tptr (Tfunction (Tcons (tptr (Tstruct _object noattr)) Tnil) tint
+              cc_default)) :: nil)
    noattr ::
  Composite _fancyfoo_object Struct
-   ((_mtable, (tptr (Tstruct _fancymethods noattr))) :: (_data, tint) ::
-    (_color, tint) :: nil)
+   (Member_plain _mtable (tptr (Tstruct _fancymethods noattr)) ::
+    Member_plain _data tint :: Member_plain _color tint :: nil)
    noattr :: nil).
 
 Definition global_definitions : list (ident * globdef fundef type) :=
-((___builtin_bswap64,
+((___compcert_va_int32,
+   Gfun(External (EF_runtime "__compcert_va_int32"
+                   (mksignature (AST.Tint :: nil) AST.Tint cc_default))
+     (Tcons (tptr tvoid) Tnil) tuint cc_default)) ::
+ (___compcert_va_int64,
+   Gfun(External (EF_runtime "__compcert_va_int64"
+                   (mksignature (AST.Tint :: nil) AST.Tlong cc_default))
+     (Tcons (tptr tvoid) Tnil) tulong cc_default)) ::
+ (___compcert_va_float64,
+   Gfun(External (EF_runtime "__compcert_va_float64"
+                   (mksignature (AST.Tint :: nil) AST.Tfloat cc_default))
+     (Tcons (tptr tvoid) Tnil) tdouble cc_default)) ::
+ (___compcert_va_composite,
+   Gfun(External (EF_runtime "__compcert_va_composite"
+                   (mksignature (AST.Tint :: AST.Tint :: nil) AST.Tint
+                     cc_default)) (Tcons (tptr tvoid) (Tcons tuint Tnil))
+     (tptr tvoid) cc_default)) ::
+ (___compcert_i64_dtos,
+   Gfun(External (EF_runtime "__compcert_i64_dtos"
+                   (mksignature (AST.Tfloat :: nil) AST.Tlong cc_default))
+     (Tcons tdouble Tnil) tlong cc_default)) ::
+ (___compcert_i64_dtou,
+   Gfun(External (EF_runtime "__compcert_i64_dtou"
+                   (mksignature (AST.Tfloat :: nil) AST.Tlong cc_default))
+     (Tcons tdouble Tnil) tulong cc_default)) ::
+ (___compcert_i64_stod,
+   Gfun(External (EF_runtime "__compcert_i64_stod"
+                   (mksignature (AST.Tlong :: nil) AST.Tfloat cc_default))
+     (Tcons tlong Tnil) tdouble cc_default)) ::
+ (___compcert_i64_utod,
+   Gfun(External (EF_runtime "__compcert_i64_utod"
+                   (mksignature (AST.Tlong :: nil) AST.Tfloat cc_default))
+     (Tcons tulong Tnil) tdouble cc_default)) ::
+ (___compcert_i64_stof,
+   Gfun(External (EF_runtime "__compcert_i64_stof"
+                   (mksignature (AST.Tlong :: nil) AST.Tsingle cc_default))
+     (Tcons tlong Tnil) tfloat cc_default)) ::
+ (___compcert_i64_utof,
+   Gfun(External (EF_runtime "__compcert_i64_utof"
+                   (mksignature (AST.Tlong :: nil) AST.Tsingle cc_default))
+     (Tcons tulong Tnil) tfloat cc_default)) ::
+ (___compcert_i64_sdiv,
+   Gfun(External (EF_runtime "__compcert_i64_sdiv"
+                   (mksignature (AST.Tlong :: AST.Tlong :: nil) AST.Tlong
+                     cc_default)) (Tcons tlong (Tcons tlong Tnil)) tlong
+     cc_default)) ::
+ (___compcert_i64_udiv,
+   Gfun(External (EF_runtime "__compcert_i64_udiv"
+                   (mksignature (AST.Tlong :: AST.Tlong :: nil) AST.Tlong
+                     cc_default)) (Tcons tulong (Tcons tulong Tnil)) tulong
+     cc_default)) ::
+ (___compcert_i64_smod,
+   Gfun(External (EF_runtime "__compcert_i64_smod"
+                   (mksignature (AST.Tlong :: AST.Tlong :: nil) AST.Tlong
+                     cc_default)) (Tcons tlong (Tcons tlong Tnil)) tlong
+     cc_default)) ::
+ (___compcert_i64_umod,
+   Gfun(External (EF_runtime "__compcert_i64_umod"
+                   (mksignature (AST.Tlong :: AST.Tlong :: nil) AST.Tlong
+                     cc_default)) (Tcons tulong (Tcons tulong Tnil)) tulong
+     cc_default)) ::
+ (___compcert_i64_shl,
+   Gfun(External (EF_runtime "__compcert_i64_shl"
+                   (mksignature (AST.Tlong :: AST.Tint :: nil) AST.Tlong
+                     cc_default)) (Tcons tlong (Tcons tint Tnil)) tlong
+     cc_default)) ::
+ (___compcert_i64_shr,
+   Gfun(External (EF_runtime "__compcert_i64_shr"
+                   (mksignature (AST.Tlong :: AST.Tint :: nil) AST.Tlong
+                     cc_default)) (Tcons tulong (Tcons tint Tnil)) tulong
+     cc_default)) ::
+ (___compcert_i64_sar,
+   Gfun(External (EF_runtime "__compcert_i64_sar"
+                   (mksignature (AST.Tlong :: AST.Tint :: nil) AST.Tlong
+                     cc_default)) (Tcons tlong (Tcons tint Tnil)) tlong
+     cc_default)) ::
+ (___compcert_i64_smulh,
+   Gfun(External (EF_runtime "__compcert_i64_smulh"
+                   (mksignature (AST.Tlong :: AST.Tlong :: nil) AST.Tlong
+                     cc_default)) (Tcons tlong (Tcons tlong Tnil)) tlong
+     cc_default)) ::
+ (___compcert_i64_umulh,
+   Gfun(External (EF_runtime "__compcert_i64_umulh"
+                   (mksignature (AST.Tlong :: AST.Tlong :: nil) AST.Tlong
+                     cc_default)) (Tcons tulong (Tcons tulong Tnil)) tulong
+     cc_default)) ::
+ (___builtin_bswap64,
    Gfun(External (EF_builtin "__builtin_bswap64"
                    (mksignature (AST.Tlong :: nil) AST.Tlong cc_default))
      (Tcons tulong Tnil) tulong cc_default)) ::
@@ -820,91 +911,14 @@ Definition global_definitions : list (ident * globdef fundef type) :=
    Gfun(External (EF_builtin "__builtin_va_end"
                    (mksignature (AST.Tint :: nil) AST.Tvoid cc_default))
      (Tcons (tptr tvoid) Tnil) tvoid cc_default)) ::
- (___compcert_va_int32,
-   Gfun(External (EF_external "__compcert_va_int32"
-                   (mksignature (AST.Tint :: nil) AST.Tint cc_default))
-     (Tcons (tptr tvoid) Tnil) tuint cc_default)) ::
- (___compcert_va_int64,
-   Gfun(External (EF_external "__compcert_va_int64"
-                   (mksignature (AST.Tint :: nil) AST.Tlong cc_default))
-     (Tcons (tptr tvoid) Tnil) tulong cc_default)) ::
- (___compcert_va_float64,
-   Gfun(External (EF_external "__compcert_va_float64"
-                   (mksignature (AST.Tint :: nil) AST.Tfloat cc_default))
-     (Tcons (tptr tvoid) Tnil) tdouble cc_default)) ::
- (___compcert_va_composite,
-   Gfun(External (EF_external "__compcert_va_composite"
+ (___builtin_unreachable,
+   Gfun(External (EF_builtin "__builtin_unreachable"
+                   (mksignature nil AST.Tvoid cc_default)) Tnil tvoid
+     cc_default)) ::
+ (___builtin_expect,
+   Gfun(External (EF_builtin "__builtin_expect"
                    (mksignature (AST.Tint :: AST.Tint :: nil) AST.Tint
-                     cc_default)) (Tcons (tptr tvoid) (Tcons tuint Tnil))
-     (tptr tvoid) cc_default)) ::
- (___compcert_i64_dtos,
-   Gfun(External (EF_runtime "__compcert_i64_dtos"
-                   (mksignature (AST.Tfloat :: nil) AST.Tlong cc_default))
-     (Tcons tdouble Tnil) tlong cc_default)) ::
- (___compcert_i64_dtou,
-   Gfun(External (EF_runtime "__compcert_i64_dtou"
-                   (mksignature (AST.Tfloat :: nil) AST.Tlong cc_default))
-     (Tcons tdouble Tnil) tulong cc_default)) ::
- (___compcert_i64_stod,
-   Gfun(External (EF_runtime "__compcert_i64_stod"
-                   (mksignature (AST.Tlong :: nil) AST.Tfloat cc_default))
-     (Tcons tlong Tnil) tdouble cc_default)) ::
- (___compcert_i64_utod,
-   Gfun(External (EF_runtime "__compcert_i64_utod"
-                   (mksignature (AST.Tlong :: nil) AST.Tfloat cc_default))
-     (Tcons tulong Tnil) tdouble cc_default)) ::
- (___compcert_i64_stof,
-   Gfun(External (EF_runtime "__compcert_i64_stof"
-                   (mksignature (AST.Tlong :: nil) AST.Tsingle cc_default))
-     (Tcons tlong Tnil) tfloat cc_default)) ::
- (___compcert_i64_utof,
-   Gfun(External (EF_runtime "__compcert_i64_utof"
-                   (mksignature (AST.Tlong :: nil) AST.Tsingle cc_default))
-     (Tcons tulong Tnil) tfloat cc_default)) ::
- (___compcert_i64_sdiv,
-   Gfun(External (EF_runtime "__compcert_i64_sdiv"
-                   (mksignature (AST.Tlong :: AST.Tlong :: nil) AST.Tlong
-                     cc_default)) (Tcons tlong (Tcons tlong Tnil)) tlong
-     cc_default)) ::
- (___compcert_i64_udiv,
-   Gfun(External (EF_runtime "__compcert_i64_udiv"
-                   (mksignature (AST.Tlong :: AST.Tlong :: nil) AST.Tlong
-                     cc_default)) (Tcons tulong (Tcons tulong Tnil)) tulong
-     cc_default)) ::
- (___compcert_i64_smod,
-   Gfun(External (EF_runtime "__compcert_i64_smod"
-                   (mksignature (AST.Tlong :: AST.Tlong :: nil) AST.Tlong
-                     cc_default)) (Tcons tlong (Tcons tlong Tnil)) tlong
-     cc_default)) ::
- (___compcert_i64_umod,
-   Gfun(External (EF_runtime "__compcert_i64_umod"
-                   (mksignature (AST.Tlong :: AST.Tlong :: nil) AST.Tlong
-                     cc_default)) (Tcons tulong (Tcons tulong Tnil)) tulong
-     cc_default)) ::
- (___compcert_i64_shl,
-   Gfun(External (EF_runtime "__compcert_i64_shl"
-                   (mksignature (AST.Tlong :: AST.Tint :: nil) AST.Tlong
-                     cc_default)) (Tcons tlong (Tcons tint Tnil)) tlong
-     cc_default)) ::
- (___compcert_i64_shr,
-   Gfun(External (EF_runtime "__compcert_i64_shr"
-                   (mksignature (AST.Tlong :: AST.Tint :: nil) AST.Tlong
-                     cc_default)) (Tcons tulong (Tcons tint Tnil)) tulong
-     cc_default)) ::
- (___compcert_i64_sar,
-   Gfun(External (EF_runtime "__compcert_i64_sar"
-                   (mksignature (AST.Tlong :: AST.Tint :: nil) AST.Tlong
-                     cc_default)) (Tcons tlong (Tcons tint Tnil)) tlong
-     cc_default)) ::
- (___compcert_i64_smulh,
-   Gfun(External (EF_runtime "__compcert_i64_smulh"
-                   (mksignature (AST.Tlong :: AST.Tlong :: nil) AST.Tlong
-                     cc_default)) (Tcons tlong (Tcons tlong Tnil)) tlong
-     cc_default)) ::
- (___compcert_i64_umulh,
-   Gfun(External (EF_runtime "__compcert_i64_umulh"
-                   (mksignature (AST.Tlong :: AST.Tlong :: nil) AST.Tlong
-                     cc_default)) (Tcons tulong (Tcons tulong Tnil)) tulong
+                     cc_default)) (Tcons tint (Tcons tint Tnil)) tint
      cc_default)) ::
  (___builtin_fmax,
    Gfun(External (EF_builtin "__builtin_fmax"
@@ -995,20 +1009,21 @@ Definition public_idents : list ident :=
  ___builtin_read32_reversed :: ___builtin_read16_reversed ::
  ___builtin_fnmsub :: ___builtin_fnmadd :: ___builtin_fmsub ::
  ___builtin_fmadd :: ___builtin_fmin :: ___builtin_fmax ::
- ___compcert_i64_umulh :: ___compcert_i64_smulh :: ___compcert_i64_sar ::
- ___compcert_i64_shr :: ___compcert_i64_shl :: ___compcert_i64_umod ::
- ___compcert_i64_smod :: ___compcert_i64_udiv :: ___compcert_i64_sdiv ::
- ___compcert_i64_utof :: ___compcert_i64_stof :: ___compcert_i64_utod ::
- ___compcert_i64_stod :: ___compcert_i64_dtou :: ___compcert_i64_dtos ::
- ___compcert_va_composite :: ___compcert_va_float64 ::
- ___compcert_va_int64 :: ___compcert_va_int32 :: ___builtin_va_end ::
+ ___builtin_expect :: ___builtin_unreachable :: ___builtin_va_end ::
  ___builtin_va_copy :: ___builtin_va_arg :: ___builtin_va_start ::
  ___builtin_membar :: ___builtin_annot_intval :: ___builtin_annot ::
  ___builtin_sel :: ___builtin_memcpy_aligned :: ___builtin_sqrt ::
  ___builtin_fsqrt :: ___builtin_fabsf :: ___builtin_fabs ::
  ___builtin_ctzll :: ___builtin_ctzl :: ___builtin_ctz :: ___builtin_clzll ::
  ___builtin_clzl :: ___builtin_clz :: ___builtin_bswap16 ::
- ___builtin_bswap32 :: ___builtin_bswap :: ___builtin_bswap64 :: nil).
+ ___builtin_bswap32 :: ___builtin_bswap :: ___builtin_bswap64 ::
+ ___compcert_i64_umulh :: ___compcert_i64_smulh :: ___compcert_i64_sar ::
+ ___compcert_i64_shr :: ___compcert_i64_shl :: ___compcert_i64_umod ::
+ ___compcert_i64_smod :: ___compcert_i64_udiv :: ___compcert_i64_sdiv ::
+ ___compcert_i64_utof :: ___compcert_i64_stof :: ___compcert_i64_utod ::
+ ___compcert_i64_stod :: ___compcert_i64_dtou :: ___compcert_i64_dtos ::
+ ___compcert_va_composite :: ___compcert_va_float64 ::
+ ___compcert_va_int64 :: ___compcert_va_int32 :: nil).
 
 Definition prog : Clight.program := 
   mkprogram composites global_definitions public_idents _main Logic.I.
